Spec.cbor_map_sort_correct

pulse/share/steel/examples/pulse/dice/cbor/CBOR.Spec.Map.fst
@@ -76,3 +76,449 @@ let rec list_sorted_map_entry_order_no_repeats
     list_sorted_map_entry_order_no_repeats key_order q;
     list_sorted_map_entry_order_not_memP_tail key_order a q
 
+let rec list_tot_for_all_order_trans
+    (#t1: Type)
+    (order: t1 -> t1 -> bool {
+      (forall x . order x x == false) /\
+      (forall x y z . (order x y /\ order y z) ==> order x z)
+    })
+    (k1v1: _)
+    (k2v2: _)
+    (l1: list t1)
+  : Lemma
+  (requires (order k1v1 k2v2 /\
+    List.Tot.for_all (order k2v2) l1
+  ))
+  (ensures (
+    List.Tot.for_all (order k1v1) l1
+  ))
+  (decreases l1)
+= match l1 with
+  | [] -> ()
+  | _ :: q -> list_tot_for_all_order_trans order k1v1 k2v2 q
+
+let rec list_ghost_assoc
+  (#key: Type)
+  (#value: Type)
+  (k: key)
+  (m: list (key & value))
+: GTot (option value)
+  (decreases m)
+= match m with
+  | [] -> None
+  | (k', v') :: m' ->
+    if FStar.StrongExcludedMiddle.strong_excluded_middle (k == k')
+    then Some v'
+    else list_ghost_assoc k m'
+
+let rec list_ghost_assoc_append
+    (#tk #tv: Type)
+    (k: tk)
+    (l1 l2: list (tk & tv))
+: Lemma
+    (ensures (list_ghost_assoc k (l1 `List.Tot.append` l2) == (
+        match list_ghost_assoc k l1 with
+        | Some v -> Some v
+        | None -> list_ghost_assoc k l2
+    )))
+    (decreases l1)
+= match l1 with
+| [] -> ()
+| (k1, _ ) :: q1 ->
+    if FStar.StrongExcludedMiddle.strong_excluded_middle (k == k1)
+    then ()
+    else list_ghost_assoc_append k q1 l2
+
+let rec list_ghost_assoc_mem_intro
+  (#tk #tv: Type)
+  (k: tk)
+  (v: tv)
+  (l: list (tk & tv))
+: Lemma
+  (requires (list_ghost_assoc k l == Some v))
+  (ensures (List.Tot.memP (k, v) l))
+  (decreases l)
+= let (k', v') :: l' = l in
+  if FStar.StrongExcludedMiddle.strong_excluded_middle (k == k')
+  then ()
+  else list_ghost_assoc_mem_intro k v l'
+
+let rec list_ghost_assoc_no_repeats_mem_elim
+  (#tk #tv: Type)
+  (k: tk)
+  (v: tv)
+  (l: list (tk & tv))
+: Lemma
+  (requires (
+    List.Tot.no_repeats_p (List.Tot.map fst l) /\
+    List.Tot.memP (k, v) l
+  ))
+  (ensures (list_ghost_assoc k l == Some v))
+  (decreases l)
+= List.Tot.memP_map_intro fst (k, v) l;
+  let (k', v') :: l' = l in
+  if FStar.StrongExcludedMiddle.strong_excluded_middle (k == k')
+  then
+    if FStar.StrongExcludedMiddle.strong_excluded_middle (v == v')
+    then ()
+    else List.Tot.memP_map_intro fst (k, v) l'
+  else list_ghost_assoc_no_repeats_mem_elim k v l'
+
+let list_ghost_assoc_no_repeats_mem
+  (#tk #tv: Type)
+  (l: list (tk & tv))
+  (k: tk)
+  (v: tv)
+: Lemma
+  (ensures (List.Tot.no_repeats_p (List.Tot.map fst l) ==> (list_ghost_assoc k l == Some v <==> List.Tot.memP (k, v) l)))
+= Classical.move_requires (list_ghost_assoc_no_repeats_mem_elim k v) l;
+  Classical.move_requires (list_ghost_assoc_mem_intro k v) l
+
+let list_ghost_assoc_no_repeats_equiv'
+  (#tk #tv: Type)
+  (l1 l2: list (tk & tv))
+  (k: tk)
+: Lemma
+  (requires (
+    List.Tot.no_repeats_p (List.Tot.map fst l1) /\
+    List.Tot.no_repeats_p (List.Tot.map fst l2) /\
+    (forall kv . List.Tot.memP kv l1 <==> List.Tot.memP kv l2)
+  ))
+  (ensures (list_ghost_assoc k l1 == list_ghost_assoc k l2))
+= match list_ghost_assoc k l1 with
+  | None ->
+    begin match list_ghost_assoc k l2 with
+    | None -> ()
+    | Some v ->
+      list_ghost_assoc_no_repeats_mem l2 k v;
+      list_ghost_assoc_no_repeats_mem l1 k v
+    end
+  | Some v ->
+    list_ghost_assoc_no_repeats_mem l1 k v;
+    list_ghost_assoc_no_repeats_mem l2 k v
+
+let list_ghost_assoc_no_repeats_equiv
+  (#tk #tv: Type)
+  (l1 l2: list (tk & tv))
+: Lemma
+  (requires (
+    List.Tot.no_repeats_p (List.Tot.map fst l1) /\
+    List.Tot.no_repeats_p (List.Tot.map fst l2) /\
+    (forall kv . List.Tot.memP kv l1 <==> List.Tot.memP kv l2)
+  ))
+  (ensures (forall k . list_ghost_assoc k l1 == list_ghost_assoc k l2))
+= Classical.forall_intro (Classical.move_requires (list_ghost_assoc_no_repeats_equiv' l1 l2))
+
+[@@noextract_to "krml"] noextract
+let rec map_sort_merge
+  (#t1 #t2: Type)
+  (key_compare: t1 -> t1 -> int)
+  (accu: list (t1 & t2))
+  (l1: list (t1 & t2))
+  (l2: list (t1 & t2))
+: Tot (bool & list (t1 & t2))
+  (decreases (List.Tot.length l1 + List.Tot.length l2))
+= match l1, l2 with
+  |  (k1, v1) :: l1', (k2, v2) :: l2' ->
+    begin let c = key_compare k1 k2 in
+      if c = 0
+      then (false, accu `List.Tot.append` (l1 `List.Tot.append` l2))
+      else if c < 0
+      then map_sort_merge key_compare (accu `List.Tot.append` [(k1, v1)]) l1' l2
+      else
+        map_sort_merge key_compare (accu `List.Tot.append` [(k2, v2)]) l1 l2'
+        // TODO in this case:
+        // 1. prove that the sort is stable, i.e. that the maps are extensionally equal throughout
+        // 2. extract and swap the whole prefix of l2 less than the head of l1, rather than just the head of l2
+     end
+  | [], _ -> (true, accu `List.Tot.append` l2)
+  | _, [] -> (true, accu `List.Tot.append` l1)
+
+let rec list_sorted_append_elim
+  (#t: Type)
+  (order: t -> t -> bool)
+  (l1 l2: list t)
+: Lemma
+  (requires (List.Tot.sorted order (l1 `List.Tot.append` l2)))
+  (ensures (
+    List.Tot.sorted order l1 /\
+    List.Tot.sorted order l2
+  ))
+  (decreases l1)
+= match l1 with
+  | [] -> ()
+  | [_] -> ()
+  | a :: b :: q ->
+    list_sorted_append_elim order (b :: q) l2
+
+let rec list_sorted_append_chunk_intro
+  (#t: Type)
+  (order: t -> t -> bool)
+  (l1 l2 l3: list t)
+: Lemma
+  (requires (
+    List.Tot.sorted order (l1 `List.Tot.append` l2) /\
+    List.Tot.sorted order (l2 `List.Tot.append` l3) /\
+    Cons? l2
+  ))
+  (ensures (
+    List.Tot.sorted order (l1 `List.Tot.append` (l2 `List.Tot.append` l3))
+  ))
+  (decreases l1)
+= match l1 with
+  | [] -> ()
+  | [a] -> () // because of List.Tot.sorted (l2 `List.Tot.append` l3) and Cons? l2
+  | a :: l1' -> list_sorted_append_chunk_intro order l1' l2 l3
+
+let rec list_sorted_order_elim
+  (#t: Type)
+  (order: t -> t -> bool)
+  (l0: list t)
+  (a1: t)
+  (l1: list t)
+  (a2: t)
+  (l2: list t)
+: Lemma
+  (requires (
+    (forall x y z . (order x y /\ order y z) ==> order x z) /\
+    List.Tot.sorted order (l0 `List.Tot.append` (a1 :: (l1 `List.Tot.append` (a2 :: l2))))
+  ))
+  (ensures (order a1 a2 == true))
+  (decreases (List.Tot.length l0 + List.Tot.length l1))
+= match l0 with
+  | [] ->
+    begin match l1 with
+    | [] -> ()
+    | a1' :: l1' ->
+      list_sorted_order_elim order [] a1' l1' a2 l2 // and transitivity
+    end
+  | a0 :: l0' ->
+    list_sorted_order_elim order l0' a1 l1 a2 l2
+
+let rec list_sorted_append_chunk_elim
+  (#t: Type)
+  (order: t -> t -> bool)
+  (l1 l2 l3: list t)
+: Lemma
+  (requires (
+    (forall x y z . (order x y /\ order y z) ==> order x z) /\
+    List.Tot.sorted order (l1 `List.Tot.append` (l2 `List.Tot.append` l3))
+  ))
+  (ensures (
+    List.Tot.sorted order (l1 `List.Tot.append` l3)
+  ))
+  (decreases l1)
+= match l1 with
+  | [] -> list_sorted_append_elim order l2 l3
+  | [a] ->
+    begin match l3 with
+    | [] -> ()
+    | b :: q ->
+      list_sorted_append_elim order l2 l3;
+      list_sorted_order_elim order [] a l2 b q
+    end
+  | _ :: l1' -> list_sorted_append_chunk_elim order l1' l2 l3
+
+let rec map_sort_merge_correct
+  (#t1 #t2: Type)
+  (key_order: t1 -> t1 -> bool)
+  (key_compare: t1 -> t1 -> int)
+  (accu: list (t1 & t2))
+  (l1: list (t1 & t2))
+  (l2: list (t1 & t2))
+: Lemma
+  (requires (
+    (forall x . key_order x x == false) /\
+    (forall x y z . (key_order x y /\ key_order y z) ==> key_order x z) /\
+    (forall x y . key_order x y == (key_compare x y < 0)) /\
+    (forall x y . key_compare x y == 0 <==> x == y) /\
+    (forall x y . (key_compare x y < 0 <==> key_compare y x > 0)) /\
+    List.Tot.sorted (map_entry_order key_order _) (accu `List.Tot.append` l1) /\
+    List.Tot.sorted (map_entry_order key_order _) (accu `List.Tot.append` l2)
+  ))
+  (ensures (
+    let (sorted, res) = map_sort_merge key_compare accu l1 l2 in
+    (forall x . List.Tot.memP x res <==> List.Tot.memP x (accu `List.Tot.append` (l1 `List.Tot.append` l2))) /\
+    (List.Tot.no_repeats_p (List.Tot.map fst res) <==> List.Tot.no_repeats_p (List.Tot.map fst (accu `List.Tot.append` (l1 `List.Tot.append` l2)))) /\
+    (if sorted
+    then List.Tot.sorted (map_entry_order key_order _) res
+    else ~ (List.Tot.no_repeats_p (List.Tot.map fst res))
+    )
+  ))
+  (decreases (List.Tot.length l1 + List.Tot.length l2))
+= match l1, l2 with
+  | [], _ -> ()
+  | _, [] -> List.Tot.append_l_nil l1
+  | (k1, v1) :: l1', (k2, v2) :: l2' ->
+    List.Tot.map_append fst l1 l2;
+    List.Tot.map_append fst accu (l1 `List.Tot.append` l2);
+    let c = key_compare k1 k2 in
+    if c = 0
+    then
+      List.Tot.no_repeats_p_false_intro (List.Tot.map fst accu) [k1] (List.Tot.map fst l1') (List.Tot.map fst l2')
+    else if c < 0
+    then begin
+      let accu' = accu `List.Tot.append` [(k1, v1)] in
+      List.Tot.append_assoc accu l1 l2;
+      List.Tot.append_assoc accu [(k1, v1)] l1';
+      List.Tot.append_assoc accu' l1' l2;
+      List.Tot.append_assoc accu [(k1, v1)] l2;
+      list_sorted_append_elim (map_entry_order key_order _) accu' l1';
+      list_sorted_append_elim (map_entry_order key_order _) accu l2;
+      list_sorted_append_chunk_intro (map_entry_order key_order _) accu [(k1, v1)] l2;
+      map_sort_merge_correct key_order key_compare accu' l1' l2
+    end
+    else begin
+      let accu' = accu `List.Tot.append` [(k2, v2)] in
+      List.Tot.append_memP_forall l1 l2;
+      List.Tot.append_memP_forall accu (l1 `List.Tot.append` l2);
+      List.Tot.append_memP_forall accu [(k2, v2)];
+      List.Tot.append_memP_forall l1 l2';
+      List.Tot.append_memP_forall accu' (l1 `List.Tot.append` l2');
+      List.Tot.no_repeats_p_append_permut (List.Tot.map fst accu) [k2] (List.Tot.map fst l1) [] (List.Tot.map fst l2');
+      List.Tot.append_assoc (List.Tot.map fst accu) [k2] (List.Tot.map fst l1 `List.Tot.append` List.Tot.map fst l2');
+      List.Tot.map_append fst accu [(k2, v2)];
+      List.Tot.map_append fst l1 l2';
+      List.Tot.map_append fst accu' (l1 `List.Tot.append` l2');
+      List.Tot.append_assoc accu [(k2, v2)] l2';
+      list_sorted_append_elim (map_entry_order key_order _) accu' l2';
+      list_sorted_append_elim (map_entry_order key_order _) accu l1;
+      list_sorted_append_chunk_intro (map_entry_order key_order _) accu [(k2, v2)] l1;
+      List.Tot.append_assoc accu [(k2, v2)] l1;
+      map_sort_merge_correct key_order key_compare accu' l1 l2'
+    end
+
+let rec list_splitAt_length
+  (#t: Type)
+  (n: nat)
+  (l: list t)
+: Lemma
+  (requires (List.Tot.length l >= n))
+  (ensures (
+    let (l1, l2) = List.Tot.splitAt n l in
+    List.Tot.length l1 == n /\
+    List.Tot.length l1 + List.Tot.length l2 == List.Tot.length l
+  ))
+  [SMTPat (List.Tot.splitAt n l)]
+= if n = 0 then () else list_splitAt_length (n - 1) (List.Tot.tl l)
+
+let rec list_splitAt_append
+  (#t: Type)
+  (n: nat)
+  (l: list t)
+: Lemma
+  (ensures (let (l1, l2) = List.Tot.splitAt n l in
+    l == l1 `List.Tot.append` l2
+  ))
+  [SMTPat (List.Tot.splitAt n l)]
+= match l with
+  | [] -> ()
+  | a :: q ->
+    if n = 0 then () else list_splitAt_append (n - 1) q
+
+[@@noextract_to "krml"] noextract
+let rec map_sort
+  (#t1 #t2: Type)
+  (key_compare: t1 -> t1 -> int)
+  (l: list (t1 & t2))
+: Tot (bool & list (t1 & t2))
+  (decreases (List.Tot.length l))
+= let len = List.Tot.length l in
+  if len < 2
+  then (true, l)
+  else
+    let (l1, l2) = List.Tot.splitAt (len / 2) l in
+    let (res, l1') = map_sort key_compare l1 in
+    if not res
+    then (false, l1' `List.Tot.append` l2)
+    else
+      let (res, l2') = map_sort key_compare l2 in
+      if not res
+      then (false, l1' `List.Tot.append` l2')
+      else map_sort_merge key_compare [] l1' l2'
+
+let list_memP_map_forall
+  (#t1 #t2: Type)
+  (f: t1 -> t2)
+  (l: list t1)
+: Lemma
+  (forall y . List.Tot.memP y (List.Tot.map f l) <==> (exists x . List.Tot.memP x l /\ y == f x))
+= Classical.forall_intro (fun y -> List.Tot.memP_map_elim f y l);
+  Classical.forall_intro (fun x -> List.Tot.memP_map_intro f x l)
+
+#push-options "--z3rlimit 16"
+
+#restart-solver
+let rec map_sort_correct
+  (#t1 #t2: Type)
+  (key_order: t1 -> t1 -> bool)
+  (key_compare: t1 -> t1 -> int)
+  (l: list (t1 & t2))
+: Lemma
+  (requires (
+    (forall x . key_order x x == false) /\
+    (forall x y z . (key_order x y /\ key_order y z) ==> key_order x z) /\
+    (forall x y . key_order x y == (key_compare x y < 0)) /\
+    (forall x y . key_compare x y == 0 <==> x == y) /\
+    (forall x y . (key_compare x y < 0 <==> key_compare y x > 0))
+  ))
+  (ensures (let (res, l') = map_sort key_compare l in
+    (forall x . List.Tot.memP x l' <==> List.Tot.memP x l) /\
+    (List.Tot.no_repeats_p (List.Tot.map fst l') <==> List.Tot.no_repeats_p (List.Tot.map fst l)) /\
+    (res == true <==> List.Tot.no_repeats_p (List.Tot.map fst l)) /\
+    (res == true ==> (
+      List.Tot.sorted (map_entry_order key_order _) l' /\
+      (forall k . list_ghost_assoc k l' == list_ghost_assoc k l)
+    ))
+  ))
+  (decreases (List.Tot.length l))
+= let len = List.Tot.length l in
+  if len < 2
+  then ()
+  else begin
+    let (l1, l2) = List.Tot.splitAt (len / 2) l in
+    List.Tot.append_memP_forall l1 l2;
+    List.Tot.map_append fst l1 l2;
+    List.Tot.no_repeats_p_append (List.Tot.map fst l1) (List.Tot.map fst l2);
+    List.Tot.append_memP_forall (List.Tot.map fst l1) (List.Tot.map fst l2);
+    list_memP_map_forall fst l1;
+    list_memP_map_forall fst l2;
+    let (res, l1') = map_sort key_compare l1 in
+    map_sort_correct key_order key_compare l1;
+    list_memP_map_forall fst l1';
+    List.Tot.append_memP_forall (List.Tot.map fst l1') (List.Tot.map fst l2);
+    List.Tot.no_repeats_p_append (List.Tot.map fst l1') (List.Tot.map fst l2);
+    List.Tot.map_append fst l1' l2;
+    List.Tot.append_memP_forall l1' l2;
+    if not res
+    then ()
+    else begin
+      let (res, l2') = map_sort key_compare l2 in
+      map_sort_correct key_order key_compare l2;
+      list_memP_map_forall fst l2';
+      List.Tot.append_memP_forall (List.Tot.map fst l1') (List.Tot.map fst l2');
+      List.Tot.no_repeats_p_append (List.Tot.map fst l1') (List.Tot.map fst l2');
+      List.Tot.map_append fst l1' l2';
+      List.Tot.append_memP_forall l1' l2';
+      if not res
+      then ()
+      else begin
+        let (res, l') = map_sort_merge key_compare [] l1' l2' in
+        assert (map_sort key_compare l == (res, l'));
+        map_sort_merge_correct key_order key_compare [] l1' l2';
+        assert (forall x . List.Tot.memP x l' <==> (List.Tot.memP x l1' \/ List.Tot.memP x l2'));
+        assert (forall x . List.Tot.memP x l' <==> List.Tot.memP x l);
+        assert (List.Tot.no_repeats_p (List.Tot.map fst l') <==> List.Tot.no_repeats_p (List.Tot.map fst l));
+        if res
+        then begin
+          assert (List.Tot.sorted (map_entry_order key_order _) l');
+          list_sorted_map_entry_order_no_repeats key_order l';
+          list_ghost_assoc_no_repeats_equiv l l';
+          assert (forall k . list_ghost_assoc k l' == list_ghost_assoc k l)
+        end
+        else ()
+      end
+    end
+  end
+
+  #pop-options
